theory/Bear/BearGame.v
@@ -1290,10 +1290,94 @@ Proof.
   - destruct m; reflexivity.
   - destruct m; simpl.
     + reflexivity.
-    + admit.
-Admitted.
+    + apply sorted_list_eq.
+      * apply insertion_sort_sorts.
+      * apply insert_sorted.
+        apply insertion_sort_sorts.
+      * intro v.
+        rewrite insert_In.
+        repeat rewrite insertion_sort_In.
+        rewrite In_remove_iff.
+        rewrite insertion_sort_In.
+        repeat rewrite in_map_iff.
+        split; intro pf.
+        -- destruct pf as [v' [Hv'1 Hv'2]].
+           rewrite insert_In in Hv'2.
+           destruct Hv'2.
+           ++ left; congruence.
+           ++ right.
+              rewrite insertion_sort_In in H1.
+              rewrite In_remove_iff in H1.
+              destruct H1; split.
+              ** intro pf; apply H1.
+                 rewrite pf in Hv'1.
+                 now apply act_inj in Hv'1.
+              ** exists ((inv x) # v).
+                 rewrite <- Hv'1 at 3.
+                 repeat rewrite <- act_comp.
+                 rewrite inv_left, inv_right.
+                 repeat rewrite act_id; now split.
+        -- exists ((inv x) # v); split.
+           ++ rewrite <- act_comp.
+              rewrite inv_right; now apply act_id.
+           ++ rewrite insert_In.
+              destruct pf.
+              ** left; rewrite <- H1.
+                 rewrite <- act_comp.
+                 rewrite inv_left; now rewrite act_id.
+              ** right.
+                 rewrite insertion_sort_In.
+                 destruct H1 as [pf [v' [Hv'1 Hv'2]]].
+                 rewrite In_remove_iff; split.
+                 --- intro; apply pf.
+                     rewrite <- H1.
+                     rewrite <- act_comp.
+                     rewrite inv_right; now rewrite act_id.
+                 --- rewrite <- Hv'1.
+                     rewrite <- act_comp.
+                     rewrite inv_left.
+                     now rewrite act_id.
+      * apply insertion_sort_NoDup.
+        apply FinFun.Injective_map_NoDup.
+        -- cbv; apply act_inj.
+        -- apply insert_NoDup.
+           ++ apply insertion_sort_NoDup.
+              apply NoDup_remove.
+              apply s.
+           ++ rewrite insertion_sort_In.
+              rewrite In_remove_iff.
+              intros [pf1 pf2].
+              apply pf1.
+              now apply h.
+      * apply insert_NoDup.
+        -- apply insertion_sort_NoDup.
+           apply NoDup_remove.
+           apply insertion_sort_NoDup.
+           apply FinFun.Injective_map_NoDup.
+           ++ cbv; apply act_inj.
+           ++ apply s.
+        -- rewrite insertion_sort_In.
+           rewrite In_remove_iff.
+           intros [pf1 pf2].
+           apply pf1.
+           f_equal; apply h.
+           rewrite insertion_sort_In in pf2.
+           rewrite in_map_iff in pf2.
+           destruct pf2 as [v [Hv1 Hv2]].
+           apply act_inj in Hv1.
+           congruence.
+Qed.
 
-Axiom cheat : forall {X}, X.
+Lemma flip_BG_State_act {G} {H} `{GroupAction G H} x s s' :
+  BG_State_act x s = s' ->
+  BG_State_act (inv x) s' = s.
+Proof.
+  intro pf.
+  apply f_equal with (f := BG_State_act (inv x)) in pf.
+  rewrite <- BG_State_act_comp in pf.
+  rewrite inv_left in pf.
+  now rewrite BG_State_act_id in pf.
+Qed.
 
 Definition Bear_Bisim {G} {H} `{GroupAction G H} :
   InvertibleBisim (BearGame G) (BearGame G).
@@ -1311,24 +1395,41 @@ Proof.
       * rewrite <- Hx in e; auto.
       * unshelve econstructor.
         -- exact (act (inv x) (b_dest b)).
-        -- apply f_equal with (f := BG_State_act (inv x)) in Hx.
-           rewrite <- BG_State_act_comp in Hx.
-           rewrite inv_left in Hx.
-           rewrite BG_State_act_id in Hx.
-           rewrite Hx.
+        -- apply flip_BG_State_act in Hx; rewrite <- Hx.
            apply act_edge.
            apply b.
-        -- apply cheat.
+        -- apply flip_BG_State_act in Hx; rewrite <- Hx.
+           simpl hunters.
+           rewrite insertion_sort_In.
+           rewrite in_map_iff.
+           intros [v [Hv1 Hv2]].
+           apply (b_dest_empty b).
+           apply act_inj in Hv1; congruence.
     + apply HunterMove.
       * rewrite <- Hx in e; auto.
       * unshelve econstructor.
         -- exact (act (inv x) (h_orig h)).
         -- exact (act (inv x) (h_dest h)).
-        -- apply cheat.
+        -- apply flip_BG_State_act in Hx; rewrite <- Hx.
+           simpl hunters.
+           rewrite insertion_sort_In.
+           rewrite in_map_iff.
+           exists (h_orig h); split; auto.
+           apply h.
         -- apply act_edge.
            apply h.
-        -- apply cheat.
-        -- apply cheat.
+        -- apply flip_BG_State_act in Hx; rewrite <- Hx.
+           intro pf.
+           apply act_inj in pf.
+           now apply h.
+        -- apply flip_BG_State_act in Hx; rewrite <- Hx.
+           simpl; intro pf.
+           rewrite insertion_sort_In in pf.
+           rewrite in_map_iff in pf.
+           destruct pf as [v [Hv1 Hv2]].
+           apply act_inj in Hv1.
+           f_equal.
+           apply h; congruence.
   - simpl; intros s m s' [x Hx].
     exists (BG_State_act x s).
     apply BG_Move_act.
@@ -1397,7 +1498,46 @@ Proof.
       * apply insertion_sort_sorts.
       * apply insert_sorted.
         apply insertion_sort_sorts.
-      * apply cheat.
+      * intro v.
+        rewrite insert_In.
+        repeat rewrite insertion_sort_In.
+        rewrite In_remove_iff.
+        rewrite insertion_sort_In.
+        repeat rewrite in_map_iff.
+        split; intro pf.
+        -- destruct pf as [v' [Hv'1 Hv'2]].
+           rewrite insert_In in Hv'2.
+           destruct Hv'2.
+           ++ left. apply f_equal with (f := act x) in H1.
+              rewrite <- act_comp in H1.
+              rewrite inv_right in H1.
+              rewrite act_id in H1; congruence.
+           ++ rewrite insertion_sort_In in H1.
+              rewrite In_remove_iff in H1; destruct H1.
+              right; split.
+              ** intro pf; apply H1.
+                 rewrite <- pf.
+                 rewrite <- Hv'1.
+                 rewrite <- act_comp.
+                 rewrite inv_left.
+                 now rewrite act_id.
+              ** exists v'; split; auto.
+        -- exists ((inv x) # v); split.
+           ++ rewrite <- act_comp.
+              rewrite inv_right.
+              apply act_id.
+           ++ rewrite insert_In.
+              destruct pf.
+              ** left; congruence.
+              ** destruct H1; right; rewrite insertion_sort_In.
+                 rewrite In_remove_iff; split.
+                 --- intro; apply H1.
+                     now apply act_inj in H3.
+                 --- destruct H2 as [v' [Hv'1 Hv'2]].
+                     rewrite <- Hv'1.
+                     rewrite <- act_comp.
+                     rewrite inv_left.
+                     now rewrite act_id.
       * apply insertion_sort_NoDup.
         apply FinFun.Injective_map_NoDup.
         -- cbv; apply act_inj.
